More_Graph.thy
@@ -881,9 +881,45 @@ lemma one_sided_matchingI:
   using assms
   by blast
 
+lemma one_sided_matching_empty[intro,simp]:
+  "one_sided_matching G {} R"
+  by (auto intro: one_sided_matchingI)
+
 lemma one_sided_matching_subgraphD: "one_sided_matching G M A \<Longrightarrow> M \<subseteq> G"
   unfolding one_sided_matching_def by blast
 
 lemma one_sided_matching_subgraphD': "one_sided_matching G M A \<Longrightarrow> e \<in> M \<Longrightarrow> e \<in> G"
   by (auto dest: one_sided_matching_subgraphD)
+
+lemma one_sided_matching_insertI:
+  assumes "{i,j} \<in> G"
+  assumes "j \<notin> Vs M"
+  assumes "i \<notin> A"
+  assumes "one_sided_matching G M A"
+  shows "one_sided_matching G (insert {i,j} M) A"
+proof (intro one_sided_matchingI)
+  from assms show "insert {i,j} M \<subseteq> G"
+    by (auto dest: one_sided_matching_subgraphD)
+next
+  fix a assume "a \<in> A"
+
+  then show "card {e \<in> insert {i,j} M. a \<in> e} \<le> 1"
+  proof (cases "a = j")
+    case True
+    with \<open>j \<notin> Vs M\<close> have "{e \<in> insert {i, j} M. a \<in> e} = {{i,j}}"
+      by (auto simp: vs_member_intro)
+
+    then show ?thesis
+      by simp
+  next
+    case False
+    with \<open>a \<in> A\<close> \<open>i \<notin> A\<close> have *: "{e \<in> insert {i,j} M. a \<in> e} = {e \<in> M. a \<in> e}"
+      by auto
+
+    with \<open>a \<in> A\<close> \<open>one_sided_matching G M A\<close> show ?thesis
+      unfolding one_sided_matching_def
+      by simp
+  qed
+qed
+
 end
